@prefix dct:   <http://purl.org/dc/terms/> .
@prefix rdf:   <http://www.w3.org/1999/02/22-rdf-syntax-ns#> .
@prefix rdfs:  <http://www.w3.org/2000/01/rdf-schema#> .
@prefix skos:  <http://www.w3.org/2004/02/skos/core#> .

<DataCommunicationMethod/voiceLandline> a skos:Concept ;
    skos:notation "voiceLandline" ;
    rdfs:label "Voice/landline"@en ,
    "Voix/ligne fixe"@fr ,
    "Voz/línea terrestre"@es ,
    "Голос/наземная линия"@ru ;
    dct:description  "Voice communications using a fixed terrestrial telecommunications network"@en ,
    "Transmission vocale à l’aide d’un réseau terrestre fixe de télécommunications"@fr ,
    "Comunicaciones por voz mediante una red de telecomunicaciones terrestre fija"@es ,
    "Голосовая связь с использованием фиксированной наземной сети связи"@ru .

<DataCommunicationMethod/voiceCellular> a skos:Concept ;
    skos:notation "voiceCellular" ;
    rdfs:label "Voice/cellular"@en ,
    "Voix/mobile"@fr ,
    "Voz/celular"@es ,
    "Голос/сотовая"@ru ;
    dct:description  "Voice communications using a cellular or similar terrestrial telecommunications network"@en ,
    "Transmission vocale à l’aide d’un réseau terrestre cellulaire ou assimilé de télécommunications"@fr ,
    "Comunicaciones por voz mediante una red de telecomunicaciones terrestre celular o similar"@es ,
    "Голосовая связь с использованием сотовой или аналогичной наземной сети связи"@ru .

<DataCommunicationMethod/voiceRadio> a skos:Concept ;
    skos:notation "voiceRadio" ;
    rdfs:label "Voice/radio"@en ,
    "Voix/radio"@fr ,
    "Voz/radio"@es ,
    "Голос/радио"@ru ;
    dct:description  "Voice communications using a direct radio system (such as VHF, HF SSB)"@en ,
    "Transmission vocale à l’aide d’un système radio direct (VHF, HF BLU, etc.)"@fr ,
    "Comunicaciones por voz mediante un sistema de radio directo (como VHF, HF BLU)"@es ,
    "Голосовая связь с использованием прямой радиосистемы (такой, как VHF, HF SSB)"@ru .

<DataCommunicationMethod/voiceSatellite> a skos:Concept ;
    skos:notation "voiceSatellite" ;
    rdfs:label "Voice/satellite"@en ,
    "Voix/satellite"@fr ,
    "Voz/satélite"@es ,
    "Голос/спутник"@ru ;
    dct:description  "Voice communications using a satellite telecommunications network"@en ,
    "Transmission vocale à l’aide d’un réseau de satellites de télécommunications"@fr ,
    "Comunicaciones por voz mediante una red de telecomunicaciones por satélite"@es ,
    "Голосовая связь с использованием спутниковой сети телесвязи"@ru .

<DataCommunicationMethod/dataLandline> a skos:Concept ;
    skos:notation "dataLandline" ;
    rdfs:label "Data/landline"@en ,
    "Données/ligne fixe"@fr ,
    "Datos/línea terrestre"@es ,
    "Данные/наземная линия"@ru ;
    dct:description  "Data communications (digital or modem) using a fixed terrestrial telecommunications network (copper or fibre)"@en ,
    "Transmission de données (par voie numérique ou modem) à l’aide d’un réseau terrestre fixe de télécommunications (cuivre ou fibre)"@fr ,
    "Comunicaciones por datos (digitales o por módem) usando una red de telecomunicaciones terrestre fija (cobre o fibra)"@es ,
    "Передача данных (цифровая или модемная) с использованием фиксированной наземной сети телесвязи (медной или фибровой оптоволоконной)"@ru .

<DataCommunicationMethod/dataCellular> a skos:Concept ;
    skos:notation "dataCellular" ;
    rdfs:label "Data/cellular"@en ,
    "Données/mobile"@fr ,
    "Datos/celular"@es ,
    "Данные/сотовая"@ru ;
    dct:description  "Data communications (digital or modem) using a cellular or similar terrestrial telecommunications network"@en ,
    "Transmission de données (par voie numérique ou modem) à l’aide d’un réseau terrestre cellulaire ou assimilé de télécommunications"@fr ,
    "Comunicaciones por datos (digitales o por módem) usando una red de telecomunicaciones terrestre celular o similar"@es ,
    "Передача данных (цифровая или модемная) с использованием сотовой или аналогичной наземной телекоммуникационной сети"@ru .

<DataCommunicationMethod/dataRadio> a skos:Concept ;
    skos:notation "dataRadio" ;
    rdfs:label "Data/radio"@en ,
    "Données/radio"@fr ,
    "Datos/radio"@es ,
    "Данные/радио"@ru ;
    dct:description  "Data communications (digital or modem) using a direct radio system (such as VHF, HF SSB, microwave)"@en ,
    "Transmission de données (par voie numérique ou modem) à l’aide d’un système radio direct (VHF, HF BLU, hyperfréquences, etc.)"@fr ,
    "Comunicaciones por datos (digitales o por módem) mediante un sistema de radio directo (como VHF, HF BLU, microondas)"@es ,
    "Передача данных (цифровая или модемная) с использованием прямой радиосистемы (такой, как VHF, HF SSB, мироволновая)"@ru .

<DataCommunicationMethod/dataSatGeostationary> a skos:Concept ;
    skos:notation "dataSatGeostationary" ;
    rdfs:label "Data/satellite/geostationary"@en ,
    "Données/satellite/géostationnaire"@fr ,
    "Datos/satélite/ geoestacionario"@es ,
    "Данные/спутник/ геостационарная"@ru ;
    dct:description  "Data communications (digital or modem) using a geostationary satellite service (such as METEOSAT)"@en ,
    "Transmission de données (par voie numérique ou modem) à l’aide d’un satellite géostationnaire (comme METEOSAT)"@fr ,
    "Comunicaciones por datos (digitales o por módem) mediante un servicio de satélite geoestacionario (como METEOSAT)"@es ,
    "Передача данных (цифровая или модемная) с использованием службы геостационарных спутников (такой, как METEOSAT)"@ru .

<DataCommunicationMethod/dataSatConstellation> a skos:Concept ;
    skos:notation "dataSatConstellation" ;
    rdfs:label "Data/satellite/constellation"@en ,
    "Données/satellite/constellation"@fr ,
    "Datos/satélite/ constelación"@es ,
    "Данные/спутник/группа спутников"@ru ;
    dct:description  "Data communications (digital or modem) using a satellite constellation service (such as IRIDIUM)"@en ,
    "Transmission de données (par voie numérique ou modem) à l’aide d’une constellation de satellites (comme IRIDIUM)"@fr ,
    "Comunicaciones por datos (digitales o por módem) mediante un servicio de constelación de satélites (como IRIDIUM)"@es ,
    "Передача данных (цифровая или модемная) с использованием службы спутниковой группы (такой, как IRIDIUM)"@ru .

<DataCommunicationMethod/dataSatIntermittent> a skos:Concept ;
    skos:notation "dataSatIntermittent" ;
    rdfs:label "Data/satellite/intermittent"@en ,
    "Données/satellite/intermittent"@fr ,
    "Datos/satélite/intermitente"@es ,
    "Данные/спутник/ промежуточный"@ru ;
    dct:description  "Data communications (digital or modem) using a satellite service with intermittent cover (such as ARGOS)"@en ,
    "Transmission de données (par voie numérique ou modem) à l’aide d’un satellite à couverture intermittente (comme ARGOS)"@fr ,
    "Comunicaciones por datos (digitales o por módem) mediante un servicio de satélite con cobertura intermitente (como ARGOS)"@es ,
    "Передача данных (цифровая или модемная) с использованием спутниковой службы с промежуточным охватом (такой, как ARGOS)"@ru .

<DataCommunicationMethod/faxLandline> a skos:Concept ;
    skos:notation "faxLandline" ;
    rdfs:label "Fax/landline"@en ,
    "Fax/ligne fixe"@fr ,
    "Fax/línea terrestre"@es ,
    "Факс/наземная линия"@ru ;
    dct:description  "Facsimile using fixed terrestrial telecommunications network"@en ,
    "Fac-similé à l’aide d’un réseau terrestre fixe de télécommunications"@fr ,
    "Facsímil usando una red de telecomunicaciones terrestre fija"@es ,
    "Факсимиле с использованием сотовой или аналогичной наземной телекоммуникационной сети"@ru .

<DataCommunicationMethod/faxCellular> a skos:Concept ;
    skos:notation "faxCellular" ;
    rdfs:label "Fax/cellular"@en ,
    "Fax/mobile"@fr ,
    "Fax/celular"@es ,
    "Факс/радио"@ru ;
    dct:description  "Facsimile using a cellular or similar terrestrial telecommunications  network"@en ,
    "Fac-similé à l’aide d’un réseau terrestre cellulaire ou assimilé de télécommunications"@fr ,
    "Facsímil usando una red de telecomunicaciones terrestre celular o similar"@es ,
    "Факсимиле с использованием радио или наналогичной наземной телекоммуникационной сети"@ru .

<DataCommunicationMethod/faxRadio> a skos:Concept ;
    skos:notation "faxRadio" ;
    rdfs:label "Fax/radio"@en ,
    "Fax/radio"@fr ,
    "Fax/radio"@es ,
    "Факс/радио"@ru ;
    dct:description  "Facsimile using a direct radio system (such as VHF, HF SSB)"@en ,
    "Fac-similé à l’aide d’un système radio direct (VHF, HF BLU, etc.)"@fr ,
    "Facsímil usando un sistema de radio directo (como VHF, HF BLU)"@es ,
    "Факсимиле с использованием прямой радиосистемы (такой, как VHF, HF SSB)"@ru .

<DataCommunicationMethod/post> a skos:Concept ;
    skos:notation "post" ;
    rdfs:label "Post"@en ,
    "Service postal"@fr ,
    "Correo"@es ,
    "Почта"@ru ;
    dct:description  "Physical transfer of information by postal, delivery service, courier service or similar"@en ,
    "Transfert physique d’informations par voie postale, service de livraison, service courrier ou assimilé"@fr ,
    "Transferencia física de información mediante servicio postal, servicio de entregas, mensajería o similares"@es ,
    "Физическая передача информации почтовой службой, службой доставки, курьерской службой или аналогичной службой"@ru .

<DataCommunicationMethod> a skos:Collection ;
        rdfs:label "Data communication method" ;
        dct:description  "Data communication method between the station/platform and some central facility. EXAMPLES:  Inmarsat-C, ARGOS, Cellular, Globalstar, GMS(DCP), Iridium, Orbcomm, VSat, landline telephone, mail "@en ;
        skos:member 

<DataCommunicationMethod/voiceLandline>,
<DataCommunicationMethod/voiceCellular>,
<DataCommunicationMethod/voiceRadio>,
<DataCommunicationMethod/voiceSatellite>,
<DataCommunicationMethod/dataLandline>,
<DataCommunicationMethod/dataCellular>,
<DataCommunicationMethod/dataRadio>,
<DataCommunicationMethod/dataSatGeostationary>,
<DataCommunicationMethod/dataSatConstellation>,
<DataCommunicationMethod/dataSatIntermittent>,
<DataCommunicationMethod/faxLandline>,
<DataCommunicationMethod/faxCellular>,
<DataCommunicationMethod/faxRadio>,
<DataCommunicationMethod/post>.
