@prefix dct:   <http://purl.org/dc/terms/> .
@prefix rdf:   <http://www.w3.org/1999/02/22-rdf-syntax-ns#> .
@prefix rdfs:  <http://www.w3.org/2000/01/rdf-schema#> .
@prefix skos:  <http://www.w3.org/2004/02/skos/core#> .

<02/igbp> a skos:Concept ;
    skos:notation "igbp" ;
    rdfs:label "Surface cover types (IGBP)"@en ,
    "Type de couverture du sol (PIGB)"@fr ,
    "Tipos de cobertura terrestre (PIGB)"@es ,
    "Типы поверхностного покрова (НПГБ)"@ru ;
    dct:description  "International Geosphere-Biosphere Programme https://lpdaac.usgs.gov/products/modis_products_table/mcd12q1"@en ,
    "Programme international géosphère-biosphère https://lpdaac.usgs.gov/products/modis_products_table/mcd12q1 "@fr ,
    "Programa Internacional Geosfera-Biosfera (PIGB) https://lpdaac.usgs.gov/products/modis_products_table/mcd12q1"@es ,
    "Международная программа геосфера/биосфера https://lpdaac.usgs.gov/products/modis_products_table/mcd12q1"@ru .

<02/umd> a skos:Concept ;
    skos:notation "umd" ;
    rdfs:label "Surface cover types (UMD)"@en ,
    "Type de couverture du sol (UMD)"@fr ,
    "Tipos de cobertura terrestre (UMD)"@es ,
    "Типы поверхностного покрова (УМД)"@ru ;
    dct:description  "The University of Maryland Department of Geography generated global land cover classification collection from 1998. http://glcf.umd.edu/data/landcover/ "@en ,
    "Classification mondiale de la couverture terrestre par le Département de géographie de l’Université du Maryland depuis 1998. http://glcf.umd.edu/data/landcover/ "@fr ,
    "El Departamento de Geografía de la Universidad de Maryland generó una recopilación de las clasificaciones de la cobertura terrestre mundial desde 1998. http://glcf.umd.edu/data/landcover/ "@es ,
    "Географический факультатет Мирилендского университета создал глобальную классификацию земного покрова с 1998 г. http://glcf.umd.edu/data/landcover/ "@ru .

<02/laifpar> a skos:Concept ;
    skos:notation "laifpar" ;
    rdfs:label "Surface cover types (LAI/fPAR)"@en ,
    "Type de couverture du sol (LAI/fPAR)"@fr ,
    "Tipos de cobertura terrestre (LAI/fPAR)"@es ,
    "Типы поверхностного покрова (ИЛП/ДФАР)"@ru ;
    dct:description  "Leaf Area Index (LAI) and Fractional Photosynthetically Active Radiation (FPAR). FPAR/LAI is the Fraction of Absorbed Photosynthetically Active radiation that a plant canopy absorbs for photosynthesis and growth in the 0.4 - 0.7nm spectral range."@en ,
    "Indice de surface foliaire (LAI) et fraction absorbée du rayonnement photosynthétiquement actif (fPAR). Fraction du rayonnement photosynthétiquement actif que le couvert végétal absorbe pour la photosynthèse et la croissance dans la plage du spectre allant de 0,4 à 0,7 nm."@fr ,
    "Índice de área foliar (LAI) y radiación activa de fotosíntesis fraccionaria (FPAR). FPAR/LAI es la fracción de radiación activa de fotosíntesis que una cobertura vegetal absorbe para la fotosíntesis y el crecimiento en el dominio espectral de 0,4 - 0,7 nm."@es ,
    "Индекс листовой поверхности (ИЛП) и Доля фотосинтетически активной радиации (ДФАР). ДФАР/ИЛП − это доля фотосинтетически поглощенной активной радиации, которая поглощается растительным покровом в процессе фотосинтеза и роста в спектральном диапазоне 0,4−0,7 нм."@ru .

<02/npp> a skos:Concept ;
    skos:notation "npp" ;
    rdfs:label "Surface cover types (NPP)"@en ,
    "Type de couverture du sol (NPP)"@fr ,
    "Tipos de cobertura terrestre (PPN)"@es ,
    "Типы поверхностного покрова (ЧПП)"@ru ;
    dct:description  "Net Primary Production (NPP) lansurfaced cover scheme"@en ,
    "Classification de la couverture terrestre selon la production primaire nette"@fr ,
    "Sistema de cobertura terrestre según la producción primaria neta (PPN)"@es ,
    "Схема классификации земного покрова на основе чистой первичной продуктивности (ЧПП)"@ru .

<02/pft> a skos:Concept ;
    skos:notation "pft" ;
    rdfs:label "Surface cover types (PFT)"@en ,
    "Type de couverture du sol (PFT)"@fr ,
    "Tipos de cobertura terrestre (TFV)"@es ,
    "Типы поверхностного покрова (ФТП)"@ru ;
    dct:description  "Plant Functional Types (PFT) surface cover scheme"@en ,
    "Classification de la couverture terrestre selon le type fonctionnel de plante"@fr ,
    "Sistema de cobertura terrestre según el tipo de vegetación funcional (TFV)"@es ,
    "Схема классификации поверхностного покрова на основе функциональных типов растений (ФТП)"@ru .

<02/lccs> a skos:Concept ;
    skos:notation "lccs" ;
    rdfs:label "Surface cover types (LCCS)"@en ,
    "Type de couverture du sol (LCCS)"@fr ,
    "Tipos de cobertura terrestre (LCCS)"@es ,
    "Типы поверхностного покрова (СКЗП)"@ru ;
    dct:description  "Land cover classification scheme (LCCS)"@en ,
    "Système de classification de la couverture terrestre"@fr ,
    "Sistema de clasificación de cubiertas de la tierra (LCCS)"@es ,
    "Схема классификации земного покрова (СКЗП)"@ru .

<02> a skos:Collection ;
        rdfs:label "Surface cover classification scheme" ;
        dct:description  "Name and reference or link to document describing the classification scheme"@en ;
        skos:member 

<02/igbp>,
<02/umd>,
<02/laifpar>,
<02/npp>,
<02/pft>,
<02/lccs>.
